dist/gcc-compatible/lib/Hacl_Streaming_HMAC_bindings.ml
@@ -135,7 +135,8 @@ module Bindings(F:Cstubs.FOREIGN) =
     let hacl_Streaming_HMAC_digest =
       foreign "Hacl_Streaming_HMAC_digest"
         ((ptr hacl_Streaming_HMAC_agile_state) @->
-           (ocaml_bytes @-> (uint32_t @-> (returning void))))
+           (ocaml_bytes @->
+              (uint32_t @-> (returning hacl_Streaming_Types_error_code))))
     let hacl_Streaming_HMAC_free =
       foreign "Hacl_Streaming_HMAC_free"
         ((ptr hacl_Streaming_HMAC_agile_state) @-> (returning void))
